Restore outputs, AND works

Bool.v
@@ -31,165 +31,47 @@ Module BoolGadget(PF: GaloisField).
   Definition andb_check :=
     <[ { (1i[0]) * (1i[1]) == (1o[0]) } ]>.  
 
-
-  Ltac deconj :=
-    repeat match goal with
-    | [H: _ /\ _ |- _ ] => invert H
-    end.
-
-  Ltac pksimpl :=
-    repeat match goal with
-           |[H: _ |- context[pkmul ?a 0:%p]] => rewrite Rmul_zero_l
-           |[H: _ |- context[pkmul 1:%p ?a]] => rewrite (Rmul_1_l (F_R FTH))
-           |[H: _ |- context[pkmul 0:%p ?a]] =>
-            replace (pkmul 0:%p a) with (pkmul a 0:%p) by (apply (Rmul_comm (F_R FTH)))
-           |[H: _ |- pksub 0:%p ?a = 0:%p] =>
-            apply Rsub_0_0
-           end.
-  
-  (** Second equivalence proof over r1cs *)
+  (** Equivalence proof over r1cs *)
   Theorem and_equiv_r1cs:
     andb <=*=> andb_check.
   Proof.    
-    unfold r1cs_lambda_tequiv, andb, andb_check.
-    intros args results inps outs vars t t' HTe Hins Houts.
-    cbn in vars.
-
-    unfold cannonical in Hins, Houts;
-    unfold correct, correct_lt;
-    split; intros HPrem;      
-      pose proof (vec2_proj inps); pose proof (vec1_proj outs);exists_inverter; deconj; subst;
-        invert HTe; cbn in H7; pick fresh x for L; specialize (H7 x Fr);
-          (** Invert inputs *)
-          pose proof (inversion_principle_bool_bool args a0 b H0 H5);
-          (** Invert outputs *)
-          invert H7.
-    - (** results :: Bool *)
-      pose proof (inversion_principle_bool results a _ H H2); invert H3; deconj.
-      + econstructor; cbn; pksimpl.
-        invert H6; deconj.
-        * rewrite (Rsub_def (F_R FTH)).
-          rewrite (Ropp_def (F_R FTH)).
-          reflexivity.
-        * solve_stlc.
-        * constructor.
-      + econstructor; cbn; pksimpl; invert H6; invert H7; deconj.
-        * solve_stlc.
-        * invert H6; deconj.
-          solve_stlc.
-          solve_stlc.
-        * pksimpl; reflexivity.
-        * invert H6; deconj.
-          pksimpl; reflexivity.
-          pksimpl; reflexivity.
-        * constructor.
-        * constructor.
-        * constructor.
-        * constructor.
-    - (** results :: Field *)
-      invert H; invert H2; invert H3; deconj.
-      solve_stlc.
-      invert H; deconj. solve_stlc.
-      invert H2; deconj; solve_stlc.
-
-    - pose proof (inversion_principle_bool_bool args a0 b H0 H5); invert H3; invert H6; deconj.
-      + econstructor.
-        beta.
-        cbn.
-        econstructor. apply step_binop_cog_1; constructor; repeat constructor.
-        econstructor. apply step_binop_cog_2; constructor; repeat constructor.
-        econstructor. apply step_and_1; constructor.
-        pose proof (inversion_principle_bool results a Datatypes.nil H H2).
-        invert H6; deconj.
-        * apply multi_refl.
-        * invert HPrem; cbn in H11.
-          repeat rewrite (Rmul_1_l (F_R FTH)) in H11.
-          rewrite (Rsub_def (F_R FTH)) in H11.
-          rewrite Ropp_0_0 in H11.
-          rewrite (Radd_comm (F_R FTH)) in H11.
-          rewrite (Radd_0_l (F_R FTH)) in H11.          
-          destruct (FTH).
-          contradiction.
-      + invert H3; deconj.
-        * destruct (FTH); contradiction.
-        * invert H6; deconj.
-          destruct (FTH); contradiction.
-          destruct (FTH); contradiction.
-      + invert H7; deconj.
-        * destruct (FTH); contradiction.
-        * invert H3; deconj; destruct (FTH); contradiction.
-      + invert H3; deconj; invert H7; deconj;
-        pose proof (inversion_principle_bool results a Datatypes.nil H H2).
-
-        * invert H7; deconj.
-          invert HPrem; cbn in H11.
-          repeat rewrite (Rmul_1_l (F_R FTH)) in H11.
-          rewrite (Rsub_def (F_R FTH)) in H11.          
-          rewrite (Radd_0_l (F_R FTH)) in H11.
-          apply Ropp_1_not_0 in H11.
-          contradiction.
-          
-          econstructor.
-          beta.
-          cbn.
-          
-          econstructor. apply step_binop_cog_1; constructor; repeat constructor.
-          econstructor. apply step_binop_cog_2; constructor; repeat constructor.
-          econstructor. apply step_and_2; constructor.
-          apply multi_refl.
-
-        * invert H6; deconj; invert H3; deconj; try (destruct FTH; contradiction).
-        * invert H3; deconj; invert H6; deconj; try (destruct FTH; contradiction).
-        * invert H7; deconj; invert H3; deconj; invert H6; deconj.
-          invert HPrem; cbn in H11.
-          
-          repeat rewrite (Rmul_1_l (F_R FTH)) in H11.
-          rewrite (Rsub_def (F_R FTH)) in H11.          
-          rewrite (Radd_0_l (F_R FTH)) in H11.
-          apply Ropp_1_not_0 in H11.
-          contradiction.
-
-          destruct FTH; contradiction.
-          destruct FTH. symmetry in H8. contradiction.
-
-          invert HPrem; cbn in H11.
-          
-          repeat rewrite (Rmul_1_l (F_R FTH)) in H11.
-          rewrite (Rsub_def (F_R FTH)) in H11.          
-          rewrite (Radd_0_l (F_R FTH)) in H11.
-          apply Ropp_1_not_0 in H11.
-          contradiction.
-
-          econstructor. beta. cbn.
-          econstructor. apply step_binop_cog_1; constructor; repeat constructor.
-          econstructor. apply step_binop_cog_2; constructor; repeat constructor.
-          econstructor. apply step_and_4; constructor.
-          apply multi_refl.
-
-          econstructor. beta. cbn.
-          econstructor. apply step_binop_cog_1; constructor; repeat constructor.
-          econstructor. apply step_binop_cog_2; constructor; repeat constructor.
-          econstructor. apply step_and_4; constructor.
-          apply multi_refl.
-          
-          destruct FTH; symmetry in H8; contradiction.
-          econstructor. beta. cbn.
-          econstructor. apply step_binop_cog_1; constructor; repeat constructor.
-          econstructor. apply step_binop_cog_2; constructor; repeat constructor.
-          econstructor. apply step_and_4; constructor.
-          apply multi_refl.
-    - (** results :: Field *)
-      invert H12.
-      invert H8.
-      invert H7.
-      invert H6.
-      invert H6.
-      Unshelve.
-      exact empty.
-      exact empty.
-      exact empty.
-      exact empty.
-      exact empty.
+    unfold r1cs_lambda_equiv, andb, andb_check.
+    intros.
+    cbn in vars, inps, outs, HcannonIn, HcannonOut.
+    unfold correct, correct_lt.
+    split; intros HPrem;
+      invert HeT; cbn in H1; pick fresh x for L; specialize (H1 x Fr); invert H1;
+        repeat invert_types; subst;
+          pose proof (vec2_proj inps); exists_inverter; deconj;
+            pose proof (vec1_proj outs); exists_inverter; deconj; subst;
+              pose proof (cannonical_forms_bool_bool args a b HcannonIn) as HcasesIn;
+              pose proof (cannonical_forms_bool result a0 HcannonOut) as HcasesOut;
+              clear HcannonIn HcannonOut.
+    - (** Backwards reasoning *)
+      deconj; econstructor; cbn; try constructor.
+      + now autorewrite with pk using trivial.
+      + now repeat invert_stlc.
+      + now repeat invert_stlc.
+      + now repeat invert_stlc.
+      + now repeat invert_stlc.
+      + now autorewrite with pk using trivial.
+      + now autorewrite with pk using trivial.
+      + now autorewrite with pk using trivial.
+    - (** Forward reasoning *)      
+      invert HPrem; deconj; cbn in H2; autorewrite with pk in H2.
+      + now repeat (try econstructor; try beta).
+      + now invert H2; apply mod_0_neq_min_1 in H0; contradiction.
+      + now invert H2; apply mod_0_neq_min_1 in H0; contradiction.
+      + now invert H2; apply mod_0_neq_min_1 in H0; contradiction.
+      + now invert H2; symmetry in H0; apply mod_0_neq_1 in H0; contradiction.
+      + now repeat (try econstructor; try beta).
+      + now repeat (try econstructor; try beta).
+      + now repeat (try econstructor; try beta).
+        Unshelve.        
+        exact empty.
+        exact empty.
+        exact empty.
+        exact empty.
   Qed.
 
   (** 2: Logical Or *)
@@ -199,180 +81,69 @@ Module BoolGadget(PF: GaloisField).
 
   (** (X1 − 1) · (1 − X2) + 1 − Y1 = 0 *)
   Definition orb_check :=
-    <[ { (1i[0] + [-1]) * ([1] + -1i[1]) == (1o[0]+[-1]) } ]>.
+    <[ { (1i[0] + [-1]) * ([1] + -1i[1]) == (1o+[-1]) } ]>.
 
   (** Second equivalence proof over r1cs *)
   Theorem or_equiv_r1cs:
     orb <=*=> orb_check.
   Proof.    
-    unfold r1cs_lambda_tequiv, orb, orb_check.
-    intros args results inps outs vars t t' HTe Hins Houts.
-    cbn in vars.
-    destruct (FTH).
-    invert F_R.
-    unfold cannonical in Hins, Houts;
-    unfold correct, correct_lt;
-    split; intros HPrem;      
-      pose proof (vec2_proj inps); pose proof (vec1_proj outs);exists_inverter; deconj; subst;
-        invert HTe; cbn in H7; pick fresh x for L; specialize (H7 x Fr);
-          (** Invert inputs *)
-          pose proof (inversion_principle_bool_bool args a0 b H0 H5);
-          (** Invert outputs *)
-          invert H7.
-    - (** results :: Bool *)
-      pose proof (inversion_principle_bool results a _ H H2); invert H3; deconj.
-      + econstructor; cbn; pksimpl.
-        invert H6; deconj.
-        * 
-          repeat rewrite <- Ropp_pkmul.
-          replace (pkplus (pkopp 1:%p) 1:%p) with (pkplus 1:%p (pkopp 1:%p)) by (apply Radd_comm).          
-          rewrite Ropp_def.
-          rewrite Rmul_comm.
-          rewrite Rplus_min1_1.
-          rewrite Rsub_def.
-          rewrite Ropp_def.
-          reflexivity.
-        * solve_stlc.
-        * constructor.
-      + econstructor; cbn; pksimpl; invert H6; invert H7; deconj.
-        * solve_stlc;
-          rewrite Rplus_min1_1;
-          rewrite Rsub_def;
-          rewrite Ropp_0_0;
-          rewrite Radd_0_l;
-          reflexivity.
-        * invert H6; deconj;
-            rewrite Rplus_min1_1;
-            rewrite Rsub_def;
-            rewrite Ropp_0_0.
-          rewrite Rmul_min1_1.
-          rewrite Radd_comm; rewrite Radd_0_l.
-          rewrite Radd_comm; rewrite Radd_0_l.
-          rewrite Radd_comm; rewrite Ropp_def.
-          rewrite Rmul_zero_l.
-          reflexivity.
-          Locate Rmul_0_l.
-          (** What are those obligations? *)
-  Admitted.
-  (**
-          cbn.
-          rewrite Rplus_min1_1.
-          rewrite 
-          solve_stlc.
-        * pksimpl; reflexivity.
-        * invert H6; deconj.
-          pksimpl; reflexivity.
-          pksimpl; reflexivity.
-        * constructor.
-        * constructor.
-        * constructor.
-        * constructor.
-    - (** results :: Field *)
-      invert H; invert H2; invert H3; deconj.
-      solve_stlc.
-      invert H; deconj. solve_stlc.
-      invert H2; deconj; solve_stlc.
-
-    - pose proof (inversion_principle_bool_bool args a0 b H0 H5); invert H3; invert H6; deconj.
+    unfold r1cs_lambda_equiv, orb, orb_check.
+    intros.
+    cbn in vars, inps, Hcannon.
+    unfold correct, correct_lt; split.
+    - (** Backwards reasoning *)
+      intros HPrem; pose proof (vec2_proj inps); exists_inverter; deconj;subst;
+        invert HeT; cbn in H1; pick fresh x for L; specialize (H1 x Fr);
+          pose proof (cannonical_forms_bool_bool args a b Hcannon) as Hcases; clear Hcannon;
+            invert Hresult; repeat invert_types; subst; destruct (FTH); inversion F_R;
+              deconj; econstructor; cbn; try constructor.
+      + now autorewrite with pk; rewrite Rmul_zero_r; reflexivity.
+      + now autorewrite with pk; rewrite Rmul_zero_r; rewrite Radd_0_l;
+        autorewrite with pk using trivial.
+      + now autorewrite with pk; rewrite Rmul_zero_r; reflexivity.
+      + now repeat invert_stlc. 
+      + now repeat invert_stlc.
+      + now repeat invert_stlc.
+      + now repeat invert_stlc.
+      + now autorewrite with pk; rewrite Rmul_zero_r; autorewrite with pk using trivial.
+    - (** Forward reasoning *)
+      intros HPrem; pose proof (vec2_proj inps); exists_inverter; deconj; subst;
+        invert HeT; invert HPrem; cbn in *; pick fresh x for L; specialize (H1 x Fr);
+          pose proof (cannonical_forms_bool_bool args a b Hcannon) as Hcases;
+            clear Hcannon; invert Hresult; repeat invert_types; subst;
+              destruct (FTH); inversion F_R; deconj; cbn; autorewrite with pk in H3.
+      + now repeat econstructor.
       + econstructor.
-        beta.
-        cbn.
-        econstructor. apply step_binop_cog_1; constructor; repeat constructor.
-        econstructor. apply step_binop_cog_2; constructor; repeat constructor.
-        econstructor. apply step_and_1; constructor.
-        pose proof (inversion_principle_bool results a Datatypes.nil H H2).
-        invert H6; deconj.
-        * apply multi_refl.
-        * invert HPrem; cbn in H11.
-          repeat rewrite (Rmul_1_l (F_R FTH)) in H11.
-          rewrite (Rsub_def (F_R FTH)) in H11.
-          rewrite Ropp_0_0 in H11.
-          rewrite (Radd_comm (F_R FTH)) in H11.
-          rewrite (Radd_0_l (F_R FTH)) in H11.          
-          destruct (FTH).
-          contradiction.
-      + invert H3; deconj.
-        * destruct (FTH); contradiction.
-        * invert H6; deconj.
-          destruct (FTH); contradiction.
-          destruct (FTH); contradiction.
-      + invert H7; deconj.
-        * destruct (FTH); contradiction.
-        * invert H3; deconj; destruct (FTH); contradiction.
-      + invert H3; deconj; invert H7; deconj;
-        pose proof (inversion_principle_bool results a Datatypes.nil H H2).
-
-        * invert H7; deconj.
-          invert HPrem; cbn in H11.
-          repeat rewrite (Rmul_1_l (F_R FTH)) in H11.
-          rewrite (Rsub_def (F_R FTH)) in H11.          
-          rewrite (Radd_0_l (F_R FTH)) in H11.
-          apply Ropp_1_not_0 in H11.
-          contradiction.
-          
-          econstructor.
-          beta.
-          cbn.
-          
-          econstructor. apply step_binop_cog_1; constructor; repeat constructor.
-          econstructor. apply step_binop_cog_2; constructor; repeat constructor.
-          econstructor. apply step_and_2; constructor.
-          apply multi_refl.
-
-        * invert H6; deconj; invert H3; deconj; try (destruct FTH; contradiction).
-        * invert H3; deconj; invert H6; deconj; try (destruct FTH; contradiction).
-        * invert H7; deconj; invert H3; deconj; invert H6; deconj.
-          invert HPrem; cbn in H11.
-          
-          repeat rewrite (Rmul_1_l (F_R FTH)) in H11.
-          rewrite (Rsub_def (F_R FTH)) in H11.          
-          rewrite (Radd_0_l (F_R FTH)) in H11.
-          apply Ropp_1_not_0 in H11.
-          contradiction.
-
-          destruct FTH; contradiction.
-          destruct FTH. symmetry in H8. contradiction.
-
-          invert HPrem; cbn in H11.
-          
-          repeat rewrite (Rmul_1_l (F_R FTH)) in H11.
-          rewrite (Rsub_def (F_R FTH)) in H11.          
-          rewrite (Radd_0_l (F_R FTH)) in H11.
-          apply Ropp_1_not_0 in H11.
-          contradiction.
-
-          econstructor. beta. cbn.
-          econstructor. apply step_binop_cog_1; constructor; repeat constructor.
-          econstructor. apply step_binop_cog_2; constructor; repeat constructor.
-          econstructor. apply step_and_4; constructor.
-          apply multi_refl.
-
-          econstructor. beta. cbn.
-          econstructor. apply step_binop_cog_1; constructor; repeat constructor.
-          econstructor. apply step_binop_cog_2; constructor; repeat constructor.
-          econstructor. apply step_and_4; constructor.
-          apply multi_refl.
-          
-          destruct FTH; symmetry in H8; contradiction.
-          econstructor. beta. cbn.
-          econstructor. apply step_binop_cog_1; constructor; repeat constructor.
-          econstructor. apply step_binop_cog_2; constructor; repeat constructor.
-          econstructor. apply step_and_4; constructor.
-          apply multi_refl.
-    - (** results :: Field *)
-      invert H12.
-      invert H8.
-      invert H7.
-      invert H6.
-      invert H6.
-      Unshelve.
-      exact empty.
-      exact empty.
-      exact empty.
-      exact empty.
-      exact empty.
+        apply step_beta; repeat constructor; econstructor; try intros; econstructor.
+        econstructor.
+        econstructor.
+        econstructor.
+        econstructor.
+        cbn. 
+        econstructor.
+        apply step_binop_cog_1; repeat econstructor.        
+        now econstructor; repeat constructor.
+      + now repeat (try econstructor; try beta).
+      + now autorewrite with pk in H3;
+          rewrite Rmul_zero_r in H3;
+          autorewrite with pk in H3; invert H3; apply mod_0_neq_min_1 in H0; contradiction.
+      + now autorewrite with pk in H3;
+          rewrite Rmul_zero_r in H3; rewrite Radd_0_l in H3;
+            symmetry in H3; invert H3; apply mod_0_neq_1 in H0; contradiction.
+      + now autorewrite with pk in H3;
+          rewrite Rmul_zero_r in H3; rewrite Radd_0_l in H3;
+            autorewrite with pk in H3; symmetry in H3; invert H3; apply mod_0_neq_1 in H0;
+              contradiction.
+      + now autorewrite with pk in H3;
+          rewrite Rmul_zero_r in H3; rewrite Radd_0_l in H3; symmetry in H3;
+            invert H3; apply mod_0_neq_1 in H0; contradiction.
+      + now repeat (try econstructor; try beta).
+        Unshelve.
+        exact empty.
+        exact empty.
+        exact empty.
+        exact empty.
   Qed.
-   *)
 
   Inductive curry: exp -> exp -> Prop :=
   | Curry: forall T1 T2 e, curry <{ \_: T1 * T2, e }> <{ \_: T1, \_: T2, e }>.
